ADTExamples/QueryStructure/Bags/BagsOfTuples.v
@@ -1,4 +1,4 @@
-Require Export Bags TreeBags ListBags Tuple Heading List Program.
+Require Export Bags Tuple Heading List Program.
 Require Import String_as_OT.
 Require Import Bool String OrderedTypeEx.
 
